src/proof/iam_model/common.v
@@ -17,6 +17,13 @@ Proof.
   constructor. iIntros (stk E Ψ) "HΨ". wp_auto. done.
 Qed.
 
+Lemma wp_generatePolicyID :
+  {{{ True }}}
+    @! iammodel.generatePolicyID #()
+  {{{ (policy_id : iammodel.PolicyID.t), RET #policy_id; True }}}.
+Proof.
+Admitted.
+
 Lemma wp_State__generateNewPolicyIDAndUpdate
     l used_policy_ids_l (used_policy_ids : policy_id_set) :
   {{{ l.[(iammodel.State.t), "usedPolicyIds"] ↦ used_policy_ids_l ∗
@@ -29,6 +36,33 @@ Lemma wp_State__generateNewPolicyIDAndUpdate
       used_policy_ids_l ↦$ <[policy_id := tt]> used_policy_ids
   }}}.
 Proof.
-Admitted.
+  iIntros (Φ) "(Hused_policy_ids_addr & Hused_policy_ids) HΦ".
+  wp_method_call.
+  rewrite /iammodel.State__generateNewPolicyIDAndUpdateⁱᵐᵖˡ. wp_call.
+  wp_auto.
+  set I := (
+    "Hused_policy_ids_addr" ∷ l.[(iammodel.State.t), "usedPolicyIds"] ↦ used_policy_ids_l ∗
+    "Hused_policy_ids" ∷ used_policy_ids_l ↦$ used_policy_ids
+  )%I.
+  iAssert I with "[$Hused_policy_ids_addr $Hused_policy_ids]" as "Hloop".
+  wp_for "Hloop".
+  wp_apply (wp_generatePolicyID with "[//]").
+  iIntros (policy_id) "_". wp_auto.
+  wp_apply (wp_map_lookup2 iammodel.PolicyID (go.StructType []) with
+    "[$Hused_policy_ids]").
+  iIntros "Hused_policy_ids".
+  destruct (used_policy_ids !! policy_id) as [[]|] eqn:Hlookup.
+  - rewrite Hlookup /=. wp_auto.
+    wp_for_post. iFrame.
+  - rewrite Hlookup /=. wp_auto.
+    wp_apply (wp_map_insert iammodel.PolicyID with "[$Hused_policy_ids]").
+    iIntros "Hused_policy_ids". wp_auto.
+    iApply wp_for_post_return.
+    rewrite return_val_unseal /return_val_def.
+    rewrite exception_do_unseal /exception_do_def. wp_auto.
+    iApply "HΦ". iFrame. done.
+Unshelve.
+  all: unfold iammodel.PolicyID.t; apply _.
+Qed.
 
 End proof.
